sketch privMax_reduction_2 and privMax_reduction_3

SampCert/DifferentialPrivacy/Queries/UnboundedMax/Code.lean
@@ -20,8 +20,6 @@ noncomputable section
 
 namespace SLang
 
-variable [dps : DPSystem ℕ]
-
 
 /--
 Sum over a list, clipping each element to a maximum.
@@ -43,7 +41,7 @@ Noise the constant 0 value using the abstract noise function.
 
 This looks strange, but will specialize to Lap(ε₁/ε₂, 0) in the pure DP case.
 -/
-def privNoiseZero (ε₁ ε₂ : ℕ+) : SLang ℤ := dps.noise (fun _ => 0) 1 ε₁ ε₂ []
+def privNoiseZero [dps : DPSystem ℕ] (ε₁ ε₂ : ℕ+) : SLang ℤ := dps.noise (fun _ => 0) 1 ε₁ ε₂ []
 
 /--
 privMax main loop guard
@@ -59,7 +57,7 @@ privMax main loop body
 
 Increase k, and sample the next vk
 -/
-def privMaxF (ε₁ ε₂ : ℕ+) : ℕ × ℤ -> SLang (ℕ × ℤ) :=
+def privMaxF [DPSystem ℕ] (ε₁ ε₂ : ℕ+) : ℕ × ℤ -> SLang (ℕ × ℤ) :=
   (fun (km1, _) => do
         let k := km1 + 1
         let vk <- privNoiseZero ε₁ (4 * ε₂)
@@ -69,7 +67,7 @@ def privMaxF (ε₁ ε₂ : ℕ+) : ℕ × ℤ -> SLang (ℕ × ℤ) :=
 /--
 Return the maximum element in the list, with some amount of noising.
 -/
-def privMax_eval (ε₁ ε₂ : ℕ+) (l : List ℕ) : SLang ℕ := do
+def privMax_eval [DPSystem ℕ] (ε₁ ε₂ : ℕ+) (l : List ℕ) : SLang ℕ := do
   let τ <- privNoiseZero ε₁ (2 * ε₂)
   let v0 <- privNoiseZero ε₁ (4 * ε₂)
   let r <-
@@ -87,7 +85,7 @@ privMax is a PMF.
 
 Using the Laplace mechanism, privMax is (ε₁/ε₂)-DP.
 -/
-def privMaxPMF (ε₁ ε₂ : ℕ+) (l : List ℕ) : PMF ℕ :=
+def privMaxPMF [DPSystem ℕ] (ε₁ ε₂ : ℕ+) (l : List ℕ) : PMF ℕ :=
   ⟨ privMax_eval ε₁ ε₂ l,
     sorry⟩
 
